README.md
@@ -8,7 +8,7 @@
 <p align="center">
   <a href="https://github.com/hatter6822/seLe4n/actions/workflows/lean_action_ci.yml"><img src="https://github.com/hatter6822/seLe4n/actions/workflows/lean_action_ci.yml/badge.svg?branch=main" alt="CI" /></a>
   <a href="https://github.com/hatter6822/seLe4n/actions/workflows/platform_security_baseline.yml"><img src="https://github.com/hatter6822/seLe4n/actions/workflows/platform_security_baseline.yml/badge.svg" alt="Security" /></a>
-  <img src="https://img.shields.io/badge/version-0.22.20-blue" alt="Version" />
+  <img src="https://img.shields.io/badge/version-0.22.21-blue" alt="Version" />
   <img src="https://img.shields.io/badge/Lean-v4.28.0-blueviolet" alt="Lean 4" />
   <a href="LICENSE"><img src="https://img.shields.io/badge/license-GPLv3-blue" alt="License" /></a>
 </p>
